

$$1. \begin{cases} u_{tt} = a^2 u_{xx} \\ u(t, 0) = u_x(t, l) = 0 \\ u(0, x) = \varphi(x) \quad u_t(0, x) = \psi(x) \end{cases} \quad (*)$$

解: 分离变量:  $u(t, x) = X(x)T(t)$ . 代入原方程 (\*)

$$\text{易有 } \frac{T''}{a^2 T} = \frac{X''}{X} \quad \text{设等式值为 } -\lambda$$

$$\text{则 } T'' + \lambda a^2 T = 0; \quad X'' + \lambda X = 0$$

$$\text{且 } u(t, 0) = X(0)T(t) = 0 \quad u_x(t, l) = X'(l)T(t) = 0$$

$$\therefore X(0) = 0, \quad X'(l) = 0$$

$$I: \begin{cases} X'' + \lambda X = 0 \\ X(0) = 0, \quad X'(l) = 0 \end{cases} \quad (**)$$

讨论: ①  $\lambda = 0$  时  $X'' = 0$  则  $X = Ax + B$   $X' = A$

$$\therefore B = A = 0 \quad \text{此时 } X \equiv 0 \quad \therefore \lambda \neq 0$$

$$\text{② } \lambda < 0 \text{ 时 } \text{令 } \lambda = -k^2 \quad \therefore X'' - k^2 X = 0$$

$$\text{通解 } X'' - k^2 X = 0 \text{ 为 } X = Ae^{kx} + Be^{-kx}$$

代入边界条件 (\*\*)

$$\begin{cases} A + B = 0 \\ Ake^{kl} - Bke^{-kl} = 0 \end{cases} \Rightarrow A = B = 0 \quad \therefore \lambda \neq 0$$

$$\text{③ } \lambda > 0 \text{ 时 } \text{令 } \lambda = k^2 \quad \therefore X'' + k^2 X = 0$$

$$\text{通解为 } X = A \cos kx + B \sin kx \quad \text{由于 } X(0) = 0$$

$$\therefore A = 0 \quad \text{又 } X' = kB \cos kx \quad \therefore kB \cos kl = 0$$

$$\therefore k = \frac{\frac{2n+1}{2}\pi}{l} \quad \therefore \lambda = \left( \frac{(n+\frac{1}{2})\pi}{l} \right)^2 \quad n = 0, 1, 2, \dots$$

易错处:

$$\therefore U_n(t, x) = \sum_{n=0}^{\infty} \left( C_n \cos \frac{(n+\frac{1}{2})\pi}{l} at + D_n \sin \frac{(n+\frac{1}{2})\pi}{l} at \right) \sin \frac{(n+\frac{1}{2})\pi}{l} x$$

$$C_n = \frac{2}{l} \int_0^l \varphi(\alpha) \sin \frac{(n+\frac{1}{2})\pi}{l} \alpha d\alpha$$

$$D_n = \frac{2}{(n+\frac{1}{2})\pi a} \int_0^l \psi(\alpha) \sin \frac{(n+\frac{1}{2})\pi}{l} \alpha d\alpha$$

$$2. \begin{cases} U_{tt} = a^2 U_{xx} \\ U_x(0, t) = U_x(l, t) = 0 \\ U(x, 0) = \varphi(x), U_t(x, 0) = \psi(x) \end{cases}$$

$$\therefore U(t, x) = \frac{A_0}{2} + B_0 t + \sum_{n=1}^{\infty} \left( A_n \cos \frac{n\pi a}{l} t + B_n \sin \frac{n\pi a}{l} t \right) \cos \frac{n\pi}{l} x$$

$$A_n = \frac{2}{l} \int_0^l \varphi(\alpha) \cos \frac{n\pi \alpha}{l} d\alpha \quad (n=0, 1, \dots)$$

$$B_n = \frac{2}{n\pi a} \int_0^l \psi(\alpha) \cos \frac{n\pi \alpha}{l} d\alpha \quad (n=1, 2, \dots) \quad B_0 = \frac{1}{l} \int_0^l \psi(\alpha) d\alpha$$

$$3. \begin{cases} U_{tt} = a^2 U_{xx} \\ U_x(0, t) = U_x(l, t) = 0 \\ U(x, 0) = \varphi(x), U_t(x, 0) = \psi(x) \end{cases}$$

$$\therefore U(t, x) = \sum_{n=0}^{\infty} \left( A_n \cos \frac{(n+\frac{1}{2})\pi}{l} at + B_n \sin \frac{(n+\frac{1}{2})\pi}{l} at \right) \cos \frac{(n+\frac{1}{2})\pi}{l} x$$

$$A_n = \frac{2}{l} \int_0^l \varphi(\alpha) \cos \frac{(n+\frac{1}{2})\pi}{l} \alpha d\alpha$$

$$B_n = \frac{2}{(n+\frac{1}{2})\pi a} \int_0^l \psi(\alpha) \cos \frac{(n+\frac{1}{2})\pi}{l} \alpha d\alpha \quad (\text{后2个自推试下})$$